fstar/Code.fst
@@ -1,0 +1,30 @@
+module Code
+
+open RG_monad
+open RG_atomic
+module U8 = FStar.UInt8
+module U16 = FStar.UInt16
+
+let check_pre (test:state -> Type0) :
+  Rg unit state rely guarantee test (fun s0 _ s1 -> s0 == s1)
+  = ()
+
+
+let prog (_:unit) :
+  Rg unit state rely guarantee (fun _ -> True) (fun _ _ _ -> True) =
+  match cas 0us 0uy 1uy with
+  | Some v -> ()
+  | None ->
+    write 1us 42uy;
+    write 2us 43uy;
+    write 3us 44uy;
+    write 4us 55uy;
+    write 5us 6uy;
+    write 6us 6uy;
+    write 8us 6uy;
+    write 7us 6uy;
+    write 9us 6uy;
+    write 2us 6uy;
+    write 1us 6uy;
+    check_pre (fun s -> Map.sel s 0us == 1uy);
+    write 0us 0uy
