fstar/RG_atomic.fst
@@ -1,0 +1,47 @@
+module RG_atomic
+
+open RG_monad
+
+module U16 = FStar.UInt16
+module U8 = FStar.UInt8
+
+//
+
+//[@@ noextract_to "krml"]
+assume val read (k:U16.t) :
+  Rg U8.t state rely guarantee (fun _ -> True) (fun s0 v s1 -> s0 == s1 /\ Map.sel s0 k == v)
+//  = Rg?.reflect (fun s0 -> Map.sel s0 k, s0)
+
+//[@@ noextract_to "krml"]
+assume val write (k:U16.t) (v:U8.t) :
+  Rg unit state rely guarantee 
+    (fun s0 ->
+      guarantee s0 (Map.upd s0 k v)
+    ) (fun s0 _ s1 ->
+      s1 == Map.upd s0 k v
+    )
+//  = Rg?.reflect (fun s0 -> ((), Map.upd s0 k v))
+
+//[@@ noextract_to "krml"]
+assume val cas (k:U16.t) (old_v:U8.t) (new_v:U8.t) :
+  Rg (option U8.t) state rely guarantee
+    (fun s0 -> Map.sel s0 k == old_v ==> guarantee s0 (Map.upd s0 k new_v))
+    (fun s0 out s1 -> 
+      match out with
+      | None -> 
+         Map.sel s0 k == old_v /\ 
+        s1 == Map.upd s0 k new_v
+      | Some x -> 
+        Map.sel s0 k == x /\ 
+        x <> old_v /\ 
+        s0 == s1
+    )
+(*
+  = Rg?.reflect (
+    fun s0 -> 
+      if Map.sel s0 k = old_v then
+        (None, Map.upd s0 k new_v)
+      else
+        (Some (Map.sel s0 k), s0)
+  )
+*)
