fstar/RG_monad.fst
@@ -1,0 +1,166 @@
+module RG_monad
+
+open FStar.Monotonic.Pure
+module Map = FStar.Map
+module U = Utils
+
+let rg_pre (state:Type0) = state -> Type0
+let rg_post (a:Type) (state:Type0) (pre:rg_pre state) = 
+  s0:state -> a -> state -> Type0
+// I try to use s0:state -> a -> _:state{pre s0} -> Type0 but it's slow
+
+let rg_repr (a:Type) (state:Type0) (rely guarantee:U.preorder state)
+  (pre:rg_pre state) (post:rg_post a state pre) =
+  s0:state ->
+    Div (a & state) (pre s0) (fun out -> post s0 out._1 out._2) //  /\ U.closure (fun x y -> rely x y \/ guarantee x y) s0 out._2)
+
+unfold let rg_return_pre (state:Type0) :
+  rg_pre state = fun _ -> True
+
+unfold let rg_return_post (a:Type) (x:a) (state:Type0) :
+  rg_post a state (rg_return_pre state) 
+  = fun s0 y s1 -> s0 == s1 /\ x == y
+
+let rg_return (a:Type) (x:a) (state:Type0)
+  (rely guarantee:U.preorder state)
+  : rg_repr a state rely guarantee
+    (rg_return_pre state) (rg_return_post a x state)
+  = fun s0 -> (x, s0)
+
+
+unfold let rg_bind_pre (a b:Type) (state:Type0)
+  (rely:U.preorder state)
+  (pre_f:rg_pre state)
+  (post_f:rg_post a state pre_f)
+  (pre_g:a -> rg_pre state)
+  : rg_pre state
+  = fun s0 -> pre_f s0 /\ (forall x s1 s2. post_f s0 x s1 /\ rely s1 s2 ==> pre_g x s2)
+
+unfold let rg_bind_post (a b:Type) (state:Type0)
+  (rely:U.preorder state)
+  (pre_f:rg_pre state)
+  (post_f:rg_post a state pre_f)
+  (pre_g:a -> rg_pre state)
+  (post_g:(x:a) -> rg_post b state (pre_g x))
+  : rg_post b state (rg_bind_pre a b state rely pre_f post_f pre_g)
+  = fun s0 y s3 -> exists x s1 s2. post_f s0 x s1 /\ rely s1 s2 /\ post_g x s2 y s3
+
+let rg_bind (a b:Type) (state:Type0)
+  (rely guarantee:U.preorder state)
+  (pre_f:rg_pre state)
+  (post_f:rg_post a state pre_f)
+  (pre_g:a -> rg_pre state)
+  (post_g:(x:a) -> rg_post b state (pre_g x))
+  (f:rg_repr a state rely guarantee pre_f post_f)
+  (g: (x:a) -> rg_repr b state rely guarantee (pre_g x) (post_g x))
+  : rg_repr b state rely guarantee 
+    (rg_bind_pre a b state rely pre_f post_f pre_g)
+    (rg_bind_post a b state rely pre_f post_f pre_g post_g)
+  = fun s0 -> let x, s1 = f s0 in g x s1
+
+
+let rg_subcomp (a:Type) (state:Type0)
+  (rely guarantee:U.preorder state)
+  (pre pre':rg_pre state)
+  (post:rg_post a state pre)
+  (post':rg_post a state pre')
+  (f:rg_repr a state rely guarantee pre post)
+  : Pure (rg_repr a state rely guarantee pre' post')
+    ((forall s0. pre' s0 ==> pre s0) /\ (forall s0 x s1. pre s0 /\ post s0 x s1 ==> post' s0 x s1))
+    (fun _ -> True)
+  = f
+
+
+unfold let rg_ite_pre (a:Type) (state:Type0)
+  (pre pre':rg_pre state)
+  (b:bool)
+  : rg_pre state
+  = fun s0 -> (b ==> pre s0) /\ ((~b) ==> pre' s0)
+
+unfold let rg_ite_post (a:Type) (state:Type0)
+  (pre pre':rg_pre state)
+  (post:rg_post a state pre)
+  (post':rg_post a state pre')
+  (b:bool)
+  : rg_post a state (rg_ite_pre a state pre pre' b)
+  = fun s0 x s1 -> (b ==> post s0 x s1) /\ ((~b) ==> post' s0 x s1)
+
+let rg_ite (a:Type) (state:Type0)
+  (rely guarantee:U.preorder state)
+  (pre pre':rg_pre state)
+  (post :rg_post a state pre)
+  (post':rg_post a state pre')
+  (_:rg_repr a state rely guarantee pre post)
+  (_:rg_repr a state rely guarantee pre' post')
+  (b:bool): Type =
+  rg_repr a state rely guarantee
+    (rg_ite_pre a state pre pre' b)
+    (rg_ite_post a state pre pre' post post' b)
+
+[@@ primitive_extraction]
+// reifiable
+reflectable
+effect {
+  Rg (a:Type) 
+  ([@@@effect_param]state:Type0)
+  ([@@@effect_param]rely:U.preorder state)
+  ([@@@effect_param]guarantee:U.preorder state)
+  (pre:rg_pre state)
+  (_:rg_post a state pre)
+  with
+  {
+    repr = rg_repr;
+    return = rg_return;
+    bind = rg_bind;
+    subcomp = rg_subcomp;
+    if_then_else = rg_ite
+  }
+}
+
+unfold let lift_div_pre (a:Type) (state:Type0)
+  (wp:pure_wp a) : rg_pre state =
+  elim_pure_wp_monotonicity_forall ();
+  fun _ -> wp (fun _ -> True)
+
+unfold let lift_div_post (a:Type) (state:Type0)
+  (wp:pure_wp a) : rg_post a state (lift_div_pre a state wp)
+  = elim_pure_wp_monotonicity_forall ();
+  fun s0 x s1 -> wp (fun _ -> True) /\ ~(wp (fun y -> x =!= y \/ s0 =!= s1))
+
+assume val lift_div (a:Type) (state:Type0) (rely guarantee:U.preorder state)
+  (wp:pure_wp a) (f:eqtype_as_type unit -> DIV a wp) :
+  rg_repr a state rely guarantee
+    (lift_div_pre a state wp)
+    (lift_div_post a state wp)
+(*  
+  = elim_pure_wp_monotonicity wp;
+  fun s0 -> 
+    let x = f () in 
+    x, s0
+*)
+sub_effect DIV ~> Rg = lift_div
+
+module U8 = FStar.UInt8
+module U16 = FStar.UInt16
+
+type state: Type0 = Map.t U16.t U8.t
+
+noextract
+let rely : U.preorder state =
+  fun s1 s2 -> s1 == s2 \/ ((
+    Map.sel s1 0us == 0uy \/
+    Map.sel s1 0us == 2uy
+  ) /\ (
+    Map.sel s2 0us == 0uy \/
+    Map.sel s2 0us == 2uy
+  ))
+
+noextract
+let guarantee : U.preorder state =
+  fun s1 s2 -> s1 == s2 \/ ((
+    Map.sel s1 0us == 0uy \/
+    Map.sel s1 0us == 1uy
+  ) /\ (
+    Map.sel s2 0us == 0uy \/
+    Map.sel s2 0us == 1uy
+  ))
