nix/ArduinoStar.nix
@@ -52,9 +52,9 @@ let
 
       buildInputs = [
         z3
+        pkgs.gnumake
         fstar
         karamel
-        pkgs.emacsPackages.fstar-mode
       ];
 
     FSTAR_HOME = fstar;
